TraceDL.v
@@ -1,0 +1,209 @@
+(** Section 4: Weakest Preconds*)
+
+From Coq Require Import Ensembles
+         Bool.Bool
+  Init.Nat.
+
+From BigStepSymbEx Require Import
+  Utils
+  Maps
+  Expr
+  Syntax
+  Traces.
+Import Trace.
+
+Inductive DLexpr : Type :=
+| DLTrue
+| DLFalse
+| DLNot (b:DLexpr)
+| DLAnd (b1 b2:DLexpr)
+| DLLeq (a1 a2:Aexpr)
+| DLImpl (b1 b2: DLexpr)
+| DLBox (t: Trc) (b: DLexpr).
+
+
+Notation "x –> y"  := (DLImpl x y) (in custom com at level 70, no associativity).
+Notation "[ t ] b"  := (DLBox t b) (in custom com at level 70, no associativity).
+
+Definition DLdiamond (t: Trc) (b: DLexpr) := DLNot (DLBox t (DLNot b)).
+Notation "< t > b"  := (DLdiamond t b) (in custom com at level 70, no associativity).
+
+Fixpoint DLeval (V:Valuation) (e:DLexpr) : bool :=
+  match e with
+  | DLTrue => true
+  | DLFalse => false
+  | DLNot b => negb (DLeval V b)
+  | DLAnd b1 b2 => (DLeval V b1) && (DLeval V b2)
+  | DLImpl b1 b2 => implb (DLeval V b1) (DLeval V b2)
+  | DLLeq a1 a2 => (Aeval V a1) <=? (Aeval V a2)
+  | <{[t] b}> => match denot_fun t V with
+                | None => true
+                | Some V' => DLeval V' b
+                end
+  end.
+
+Lemma DLdiamond_charact: forall V t b,
+    DLeval V <{<t> b}> = match denot_fun t V with
+                         | None => false
+                         | Some V' => DLeval V' b
+                         end.
+Proof.
+  intros.
+  cbn.
+  destruct (denot_fun t V); auto.
+  apply negb_involutive.
+Qed.
+
+Lemma DLeval_diamond: forall V t b,
+    DLeval V <{<t> b}> = true <-> (exists V', denot_fun t V = Some V' /\ DLeval V' b = true).
+Proof.
+  split; intros.
+  - cbn in H.
+    destruct (denot_fun t V).
+    + apply negb_true_iff in H.
+      apply negb_false_iff in H.
+      now exists v.
+    + discriminate.
+  - cbn.
+    now destruct H as (?V & -> & ->).
+Qed.
+
+Fixpoint DLapply (s:sub) (e:DLexpr) : DLexpr :=
+  match e with
+  | DLTrue => DLTrue
+  | DLFalse => DLFalse
+  | DLNot b => DLNot (DLapply s b)
+  | DLAnd b1 b2 => DLAnd (DLapply s b1) (DLapply s b2)
+  | DLImpl b1 b2 => DLImpl (DLapply s b1) (DLapply s b2)
+  | DLLeq a1 a2 => DLLeq (Aapply s a1) (Aapply s a2)
+  | <{[t] b}> => DLBox t (DLapply s b)
+  end.
+
+(* This is not exactly elegant, but it lets us reuse results about Beval and
+Bapply and easily restrict to non-modal formulae *)
+Fixpoint embed (b:Bexpr) : DLexpr :=
+  match b with
+  | BTrue => DLTrue
+  | BFalse => DLFalse
+  | BNot b => DLNot (embed b)
+  | BAnd b1 b2 => DLAnd (embed b1) (embed b2)
+  | BImpl b1 b2 => DLImpl (embed b1) (embed b2)
+  | BLeq a1 a2 => DLLeq a1 a2
+  end.
+
+Lemma DLeval_embed: forall b V,
+    DLeval V (embed b) = Beval V b.
+Proof.
+  induction b; intros; try easy.
+  - cbn.
+    now rewrite IHb.
+  - cbn.
+    now rewrite IHb1, IHb2.
+  - cbn.
+    now rewrite IHb1, IHb2.
+Qed.
+
+Lemma DLapply_embed: forall b s,
+    DLapply s (embed b) = embed (Bapply s b).
+Proof.
+  induction b; intros; try easy.
+  - cbn.
+    now rewrite IHb.
+  - cbn.
+    now rewrite IHb1, IHb2.
+  - cbn.
+    now rewrite IHb1, IHb2.
+Qed.
+
+(* Lemma 6 *)
+Lemma box_weakest_precond: forall t ψ V,
+    DLeval V (DLBox t (embed ψ)) = DLeval V (DLImpl (embed (PC t)) (DLapply (Sub t) (embed ψ))).
+Proof.
+  induction t; intros; cbn;
+    rewrite  DLapply_embed, 2 DLeval_embed.
+  - now rewrite Bapply_id.
+  - rewrite <- comp_subB.
+    now rewrite <- asgn_sound'.
+  - destruct (Beval V b); auto.
+    rewrite Bapply_id.
+    now rewrite DLeval_embed.
+  - PC_spec_unfold (TSeq t1 t2).
+    apply PC_spec_correct in H3, H4; subst.
+    Sub_spec_unfold  (TSeq t1 t2).
+    apply Sub_spec_correct in H5, H6; subst.
+    destruct (denot_fun t1 V) as [?V | ] eqn:?; cbn.
+    + pose proof trace_correspondence t1 V V0 as (SOUND1 &_).
+      destruct (SOUND1 Heqo) as (? & ?).
+      destruct (denot_fun t2 V0) as [?V | ] eqn:?; cbn.
+      * pose proof trace_correspondence t2 V0 as (SOUND2 &_).
+        destruct (SOUND2 Heqo0) as (? & ?).
+        specialize (IHt1 ψ V).
+        specialize (IHt2 ψ V0).
+        cbn in IHt1, IHt2.
+        cbn.
+        rewrite <- comp_subB.
+        unfold denot_sub in H3; subst.
+        rewrite H1, H5.
+        cbn.
+        rewrite DLeval_embed.
+        rewrite <- Bapply_compose.
+        unfold denot_sub.
+        now rewrite 2 comp_subB.
+      * pose proof trace_correspondence_none t2 V0 as (SOUND2 &_).
+        specialize (IHt1 ψ V).
+        specialize (IHt2 ψ V0).
+        cbn in IHt1, IHt2.
+        unfold denot_sub in H3; subst.
+        apply SOUND2 in Heqo0.
+        rewrite <- comp_subB.
+        now rewrite H1, Heqo0.
+    + pose proof trace_correspondence_none t1 V as (SOUND1 &_).
+      rewrite SOUND1; auto.
+Qed.
+
+(* Lemma 6 *)
+Lemma diamond_weakest_precond: forall t ψ V,
+    DLeval V (DLdiamond t (embed ψ)) = DLeval V (DLAnd (embed (PC t)) (DLapply (Sub t) (embed ψ))).
+Proof.
+  induction t; intros; cbn;
+    rewrite  DLapply_embed, 2 DLeval_embed.
+  - now rewrite Bapply_id, negb_involutive.
+  - rewrite <- comp_subB, <- asgn_sound'.
+    now rewrite negb_involutive.
+  - destruct (Beval V b); auto.
+    now rewrite Bapply_id, negb_involutive, DLeval_embed.
+  - PC_spec_unfold (TSeq t1 t2).
+    apply PC_spec_correct in H3, H4; subst.
+    Sub_spec_unfold  (TSeq t1 t2).
+    apply Sub_spec_correct in H5, H6; subst.
+    destruct (denot_fun t1 V) as [?V | ] eqn:?; cbn.
+    + pose proof trace_correspondence t1 V V0 as (SOUND1 &_).
+      destruct (SOUND1 Heqo) as (? & ?).
+      destruct (denot_fun t2 V0) as [?V | ] eqn:?; cbn.
+      * pose proof trace_correspondence t2 V0 as (SOUND2 &_).
+        destruct (SOUND2 Heqo0) as (? & ?).
+        specialize (IHt1 ψ V).
+        specialize (IHt2 ψ V0).
+        cbn in IHt1, IHt2.
+        cbn.
+        rewrite <- comp_subB.
+        unfold denot_sub in H3; subst.
+        rewrite H1, H5.
+        cbn.
+        rewrite negb_involutive, DLeval_embed.
+        rewrite <- Bapply_compose.
+        unfold denot_sub.
+        now rewrite 2 comp_subB.
+      * pose proof trace_correspondence_none t2 V0 as (SOUND2 &_).
+        specialize (IHt1 ψ V).
+        specialize (IHt2 ψ V0).
+        cbn in IHt1, IHt2.
+        unfold denot_sub in H3; subst.
+        apply SOUND2 in Heqo0.
+        rewrite <- comp_subB.
+        now rewrite H1, Heqo0.
+    + pose proof trace_correspondence_none t1 V as (SOUND1 &_).
+      rewrite SOUND1; auto.
+Qed.
+
+(*TODO: Prop 1? *)
